utils/theories/All_Forall.v
@@ -176,7 +176,7 @@ Section alli.
 End alli.
 
 Lemma alli_ext {A} (p q : nat -> A -> bool) n (l : list A) :
-  (forall i, p i =1 q i) ->
+  (forall i, p i ≐1 q i) ->
   alli p n l = alli q n l.
 Proof.
   intros hfg.
@@ -352,14 +352,14 @@ Proof.
     constructor; auto. now destruct (Hp a).
 Qed.
 
-Lemma forallb_ext {A} (p q : A -> bool) : p =1 q -> forallb p =1 forallb q.
+Lemma forallb_ext {A} (p q : A -> bool) : p ≐1 q -> forallb p ≐1 forallb q.
 Proof.
   intros hpq l.
   induction l; simpl; auto.
   now rewrite (hpq a) IHl.
 Qed.
 
-#[global] Instance forallb_proper {A} : Proper (`=1` ==> eq ==> eq) (@forallb A).
+#[global] Instance forallb_proper {A} : Proper (`≐1` ==> eq ==> eq) (@forallb A).
 Proof.
   intros f g Hfg ? ? ->. now apply forallb_ext.
 Qed.
